Use Why3's hash tables, finish tuples in Ty
Removed Coq impl of Hash tables - problems with OCaml weak refs

extract/IdentExtra.ml
@@ -1,0 +1,1 @@
+module Hid = Exthtbl.Make(OrderedHashed(IdentTag))
