src/util/StateMonad.v
@@ -3,81 +3,22 @@
 Require CoqBigInt.
 Require Import ErrorMonad.
 Require Import Monad.
-Require Import Hashtbl. (*NOTE: stdpp and coq-ext-lib cannot both
+Require Import CoqHashtbl. (*NOTE: stdpp and coq-ext-lib cannot both
   be imported in same file!*)
 From ExtLib Require Import Monads MonadState StateMonad EitherMonad.
 Import MonadNotation.
 
 (*We use coq-ext-lib's monads and monad transformers.
-  (TODO) THis leads to bad OCaml code, but doing it ourselves
-    is very painful.
+  However, we cannot use their notations, or else the OCaml code
+  is full of Obj.magic.
   Because we extract to mutable references (with names), we make
   each use of state a different set of definitions.
   (TODO: can we improve this and reduce duplication>)*)
 
-(*From stdpp Require Import base.*)
-
-
-
-
-(*Generalized state monad*)
-(*Definition state (s a: Type) : Type := s -> (s * a).
-Definition st_get {s: Type} : state s s := fun x => (x, x).
-Definition st_set {s: Type} (x: s) : state s unit := fun _ => (x, tt).
-Definition st_ret {s a: Type} (x: a) : state s a := fun s => (s, x).
-Definition st_bnd {s a b: Type} (f: a -> state s b) (m: state s a) : state s b :=
-  fun i =>
-    let t := m i in
-    f (snd t) (fst t).
-Definition st_listM {s a: Type} (l: list (state s a)) := listM st_ret st_bnd l.
-
-Global Instance st_ret' s : MRet (state s) := @st_ret s.
-Global Instance st_bnd' s : MBind (state s) := @st_bnd s.
-
-(*Combine multiple states*)
-(*NOTE: this is not a very good implementation, but
-  we don't want to do things generically, or else 
-  the OCaml code will have lots of Obj.magic*)
-(*TODO: generalize to (list Type)? This will give horrible
-  OCaml code most likely*)
-Definition state_multi (s1 s2 a: Type) : Type := state (s1 * s2) a.
-Definition st_get1 {s1 s2: Type} : state_multi s1 s2 s1 := fun x => (x, fst x).
-Definition st_get2 {s1 s2: Type} : state_multi s1 s2 s2 := fun x => (x, snd x).
-Definition st_set1 {s1 s2: Type} (x: s1) : state_multi s1 s2 unit :=
-  (fun y => ((x, snd y), tt)).
-Definition st_set2 {s1 s2: Type} (x: s2) : state_multi s1 s2 unit :=
-  (fun y => ((fst y, x), tt)).
-Definition st_multi_ret {s1 s2 a: Type} (x: a) : state_multi s1 s2 a := st_ret x.
-Definition st_multi_bnd {s1 s2 a b: Type} (f: a -> state_multi s1 s2 b)
-  (m: state_multi s1 s2 a) : state_multi s1 s2 b := st_bnd f m.*)
-
-(*Combine state and error handling (monad transformer)
-Require Import ErrorMonad.
-
-(*We can't do monad transformers generically or else OCaml
-  code is bad. For now, we just combine state and error, and
-  the above lets us combine multiple states
-  (This is ExceptT on state monad)*)
-Definition exceptT (s a: Type) : Type :=
-  state s (errorM a).
-Definition exceptT_ret {s a: Type} (x: a) : exceptT s a :=
-  st_ret (ret x).
-Definition exceptT_bnd {s a b: Type} (f: a -> exceptT s b)
-  (m: exceptT s a) : exceptT s b :=
-  st_bnd (fun y =>
-    match y with
-    | Normal _ z => f z
-    | Error _ e => st_ret (Error _ e)
-    end
-  )m.
-Definition exceptT_lift {s a: Type} (x: state s a) : exceptT s a :=
-  st_bnd (fun s => st_ret (ret s)) x.
-Definition exceptT_lift2 {s a: Type} (x: errorM a) : exceptT s a :=
-  st_ret x.*)
 Local Open Scope monad_scope.
 Existing Instance
      Monad_state.
-(*Mutable counter*)
+(*1. Mutable counter*)
 Definition ctr a := (state CoqBigInt.t a).
 Global Instance Monad_ctr: Monad ctr := Monad_state _.
 Global Instance MonadState_ctr : MonadState CoqBigInt.t ctr := MonadState_state _.
@@ -91,6 +32,7 @@ Definition new_ctr (i: CoqBigInt.t) : ctr unit := put i.
 (*TODO: see if notation/inlined/whatever*)
 Definition ctr_incr : ctr unit :=
   i <- ctr_get ;; ctr_set (CoqBigInt.succ i).
+
 (*2. Hash table*)
 
 Existing Instance
@@ -107,8 +49,6 @@ Definition hash_get (a: Type) : hash_st key value (hashtbl key value):= get.
 Definition hash_set (a: Type) (x: hashtbl key value) : hash_st key value unit :=
   put x.
 Definition hash_ret {a: Type} (x: a) : hash_st key value a := ret x.
-(*TODO: change to notations or don't include at all?
-  No, Need definitions for extraction*)
 Definition hash_bnd {a b: Type} (f: a -> hash_st key value b) 
   (m: hash_st key value a) : hash_st key value b := bind m f.
 Definition new_hash : hash_st key value unit := put (create_hashtbl value).
@@ -127,7 +67,6 @@ Definition hashcons_new key : hashcons_st key unit :=
 Definition hashcons_bnd {key a b} (f: a -> hashcons_st key b) (m: hashcons_st key a) :
   hashcons_st key b := bind m f.
 Definition hashcons_ret {key a} (x: a) : hashcons_st key a := ret x.
-(*TODO: if we do definitions, can we inline?*)
 Section HashCons.
 Context {key: Type} (hash: key -> CoqBigInt.t) 
   (eqb: key -> key -> bool).
@@ -146,132 +85,55 @@ Definition hashcons_incr : hashcons_st key unit :=
 Definition hashcons_list {K A : Type} (l: list (@hashcons_st K A)) :
   @hashcons_st K (list A) := listM hashcons_ret hashcons_bnd l.
 End HashCons.
-(*TODO: for now, notations*)
-
-(*Definition hashcons_st (a: Type) : Type :=
-  state_multi CoqBigInt.t (@hashtbl key) a.
-Definition hashcons_get_ctr : hashcons_st CoqBigInt.t :=
-  st_get1.
-Definition hashcons_get_hashtbl : hashcons_st (@hashtbl key) :=
-  st_get2.
-Definition hashcons_set_ctr (x: CoqBigInt.t) : hashcons_st unit :=
-  st_set1 x.
-Definition hashcons_set_hashtbl (h: @hashtbl key) : hashcons_st unit :=
-  st_set2 h.
-Definition hashcons_ret {a: Type} (d: a) : hashcons_st a :=
-  st_multi_ret d.
-Definition hashcons_bnd {A B: Type} (f: A -> hashcons_st B) 
-  (h: hashcons_st A) : hashcons_st B :=
-  st_multi_bnd f h.
-Definition hashcons_new : hashcons_st unit :=
-  fun _ => (CoqBigInt.one, create_hashtbl, tt).*)
-
-(*Because modules cannot be passed as parameters ugh*)
-(*Definition hashcons_st (a: Type) : Type :=
-  (CoqBigInt.t * @hashtbl key) -> ((CoqBigInt.t * @hashtbl key) * a).
-Definition hashcons_incr : hashcons_st unit :=
-  (fun x => (CoqBigInt.succ (fst x), snd x, tt)).
-Definition hashcons_get_ctr : hashcons_st CoqBigInt.t :=
-  fun x => (x, fst x).
-(*Idea: we need to look up hash in the table, *)
-Definition hashcons_lookup (k: key) : hashcons_st (option key) :=
-  fun x => (x, find_opt_hashtbl hash eqb (snd x) k).
-Definition hashcons_add (k: key) : hashcons_st unit :=
-  fun x => (fst x, add_hashtbl hash (snd x) k, tt).
-Definition hashcons_new : hashcons_st unit :=
-  fun _ => (CoqBigInt.one, create_hashtbl, tt).
-Definition hashcons_ret {a: Type} (d: a) : hashcons_st a := 
-  fun x => (x, d).
-Definition hashcons_bnd {A B: Type} (f: A -> hashcons_st B) 
-  (h: hashcons_st A) : hashcons_st B :=
-  fun x =>
-    let t := h x in
-    f (snd t) (fst t).*)
-(*The hack again*)
 Definition hashcons_unit key := hashcons_st key unit.
-(*Definition hashcons_list {K A : Type} (l: list (@hashcons_st K A)) :
-  @hashcons_st K (list A) :=
-  listM hashcons_ret hashcons_bnd l.*)
 
-(*Combine error handling and hashcons*)
-(*TODO: combine with above*)
-(*Really, really want to do this generically*)
-(*Maybe I will try and hopefully get OCaml to be OK
-  with it*)
-
-
-(*Monad transformers (kind of)*)
-
-(*Later, switch to Either monad from ExtLib*)
-Definition errorHashT (K A: Type) := (eitherT errtype 
+(*4. Hash Consing + Error Handling (w monad transformers)*)
+Definition errorHashconsT (K A: Type) := (eitherT errtype 
   (state (CoqBigInt.t * (hashset K))) A).
-Global Instance Monad_errorHashT K: Monad (errorHashT K) := Monad_eitherT _ (Monad_state _). 
-Global Instance MonadT_errorHashT K: MonadT (errorHashT K) (hashcons_st K) := 
+Global Instance Monad_errorHashconsT K: Monad (errorHashconsT K) := Monad_eitherT _ (Monad_state _). 
+Global Instance MonadT_errorHashconsT K: MonadT (errorHashconsT K) (hashcons_st K) := 
   MonadT_eitherT _ (Monad_state _). 
-Global Instance MonadState_errorHashT K: MonadState (CoqBigInt.t * (hashset K))
-  (errorHashT K) := MonadState_eitherT _ (Monad_state _) (MonadState_state _).
-Global Instance Exception_errorHashT K : MonadExc errtype (errorHashT K) :=
+Global Instance MonadState_errorHashconsT K: MonadState (CoqBigInt.t * (hashset K))
+  (errorHashconsT K) := MonadState_eitherT _ (Monad_state _) (MonadState_state _).
+Global Instance Exception_errorHashconsT K : MonadExc errtype (errorHashconsT K) :=
   Exception_eitherT _ (Monad_state _).
-
-(*Global Instance MonadState_hashcons_st key : 
-  MonadState (CoqBigInt.t * hashset key) (hashcons_st key) := MonadState_state _.*)
-Definition errorHash_bnd {K a b} (f: a -> errorHashT K b) (m: errorHashT K a):
-  errorHashT K b := bind m f.
-Definition errorHash_ret {K a} (x: a) : errorHashT K a := ret x.
-Definition errorHash_lift {K a} (x: hashcons_st K a) : errorHashT K a := lift x.
+Definition errorHashcons_bnd {K a b} (f: a -> errorHashconsT K b) (m: errorHashconsT K a):
+  errorHashconsT K b := bind m f.
+Definition errorHashcons_ret {K a} (x: a) : errorHashconsT K a := ret x.
+Definition errorHashcons_lift {K a} (x: hashcons_st K a) : errorHashconsT K a := lift x.
 (*TODO: do we need this?*)
-Definition errorHash_lift2 {K a} (x: errorM a) : errorHashT K a := 
+Definition errorHashcons_lift2 {K a} (x: errorM a) : errorHashconsT K a := 
   match x with
   | inl e => raise e
   | inr t => ret t
   end.
+Definition errorHashcons_list {K A: Type} (l: list (@errorHashconsT K A)) :
+ @errorHashconsT K (list A) :=
+  listM errorHashcons_ret errorHashcons_bnd l.
 
-(*Ok, we do want a monad instance for (errorM (hashcons_st A))
-  so we can use listM
-  also this is annoying haha*)
-(*Problem is doing it generically means OCaml code is bad*)
-(*For now, do 1 by 1*)
-(*Choose this order: state still exists, may have result*)
-(*Basically ExceptT on state monad*)
-(*Notation errorHashT K A := (exceptT (CoqBigInt.t * (@hashset K)) A).
-(*Names for compatibility*)
-Notation errorHash_bnd := exceptT_bnd.
-Notation errorHash_ret := exceptT_ret.
-Notation errorHash_lift := exceptT_lift.*)
-Definition errorHash_list {K A: Type} (l: list (@errorHashT K A)) :
- @errorHashT K (list A) :=
+(*5. Hash table + error handling*)
+Definition errorHashT (K V A: Type) := (eitherT errtype 
+  (state (hashtbl K V)) A).
+Global Instance Monad_errorHashT K V: Monad (errorHashT K V) := Monad_eitherT _ (Monad_state _). 
+Global Instance MonadT_errorHashT K V: MonadT (errorHashT K V) (hash_st K V) := 
+  MonadT_eitherT _ (Monad_state _). 
+Global Instance MonadState_errorHashT K V: MonadState (hashtbl K V)
+  (errorHashT K V) := MonadState_eitherT _ (Monad_state _) (MonadState_state _).
+Global Instance Exception_errorHashT K V : MonadExc errtype (errorHashT K V) :=
+  Exception_eitherT _ (Monad_state _).
+Definition errorHash_bnd {K V a b} (f: a -> errorHashT K V b) (m: errorHashT K V a):
+  errorHashT K V b := bind m f.
+Definition errorHash_ret {K V a} (x: a) : errorHashT K V a := ret x.
+Definition errorHash_lift {K V a} (x: hash_st K V a) : errorHashT K V a := 
+  lift x.
+(*TODO: do we need this?*)
+Definition errorHash_lift2 {K V a} (x: errorM a) : errorHashT K V a := 
+  match x with
+  | inl e => raise e
+  | inr t => ret t
+  end.
+Definition errorHash_list {K V A: Type} (l: list (@errorHashT K V A)) :
+ @errorHashT K V (list A) :=
   listM errorHash_ret errorHash_bnd l.
-
-(*Definitions again - see about inline/notations*)
-
-(*Definition errorHashT {K : Type} (A: Type) : Type :=
-  @hashcons_st K (errorM A).
-
-Definition errorHash_ret {K A: Type} (x: A) : @errorHashT K A :=
-  hashcons_ret (ret x).
-
-Definition errorHash_bnd {K A B: Type} (f: A -> errorHashT B) (x: errorHashT A) : 
-  @errorHashT K B :=
-  hashcons_bnd (fun y =>
-    match y with
-    | Normal _ z => f z
-    | Error _ e => hashcons_ret (Error _ e)
-    end) x.
-
-Definition errorHash_lift {K A: Type} (x: @hashcons_st K A) :
-  @errorHashT K A :=
-  hashcons_bnd (fun s => (hashcons_ret (ret s))) x.
-
-(*TODO: am I doing this right?*)
-Definition errorHash_lift2 {K A: Type} (x: errorM A) :
-  @errorHashT K A :=
-  fun s => (s, x). 
-
-Definition errorHash_list {K A: Type} (l: list (@errorHashT K A)) :
- @errorHashT K (list A) :=
-  listM errorHash_ret errorHash_bnd l.
-*)
-
-
 
 
